splitting 2-WL

Weidenbach_Book/CDCL_Two_Watched_Literals.thy
@@ -321,7 +321,7 @@ proof
         have "\<And>l L. - (l::'a literal) \<in> L \<or> l \<notin> uminus ` L"
           by force
         then show ?thesis
-          using cw(1) cw_eq w_nw(3) raw_clause_def by (metis DiffI Un_iff cw(3) f1 f2 la(2) nla 
+          using cw(1) cw_eq w_nw(3) raw_clause_def by (metis DiffI Un_iff cw(3) f1 f2 la(2) nla
             set_append twl_clause.sel(1) twl_clause.sel(2))
       qed
     qed
@@ -466,7 +466,7 @@ proof
       next
         case False
         thus ?thesis
-          by (metis (no_types, hide_lams) M_def UnE W' contra_subsetD cw(1) cw(3) cw_eq imageE 
+          by (metis (no_types, hide_lams) M_def UnE W' contra_subsetD cw(1) cw(3) cw_eq imageE
             insertI1 l list.set(2) set_append twl_clause.sel(1) twl_clause.sel(2)
             uminus_of_uminus_id w_nw(3) raw_clause_def)
       qed
@@ -570,14 +570,14 @@ abbreviation update_backtrack_lvl where
    TWL_State (raw_trail S) (raw_init_clss S) (raw_learned_clss S) k (raw_conflicting S)"
 
 abbreviation update_conflicting where
-  "update_conflicting C S \<equiv> 
+  "update_conflicting C S \<equiv>
     TWL_State (raw_trail S) (raw_init_clss S) (raw_learned_clss S) (backtrack_lvl S) C"
 
 subsection \<open>Abstract 2-WL\<close>
 
 definition tl_trail where
   "tl_trail S =
-   TWL_State (tl (raw_trail S)) (raw_init_clss S) (raw_learned_clss S) (backtrack_lvl S) 
+   TWL_State (tl (raw_trail S)) (raw_init_clss S) (raw_learned_clss S) (backtrack_lvl S)
    (raw_conflicting S)"
 
 locale abstract_twl =
@@ -594,7 +594,7 @@ locale abstract_twl =
       "no_dup (trail S) \<Longrightarrow> undefined_lit (trail S) (lit_of L) \<Longrightarrow> wf_twl_cls (trail S) C' \<Longrightarrow>
         wf_twl_cls (L # raw_trail S) (rewatch (lit_of L) S C')"
       and
-    restart_learned: "mset (restart_learned S) \<subseteq># mset (raw_learned_clss S)" -- \<open>We need 
+    restart_learned: "mset (restart_learned S) \<subseteq># mset (raw_learned_clss S)" -- \<open>We need
       @{term mset} and not @{term set} to take care of duplicates. \<close>
 begin
 
@@ -623,9 +623,9 @@ definition
   remove_cls :: "'v literal list \<Rightarrow> 'v twl_state \<Rightarrow> 'v twl_state"
 where
   "remove_cls C S =
-   TWL_State (raw_trail S) 
+   TWL_State (raw_trail S)
      (removeAll_cond (\<lambda>D. mset (raw_clause D) = mset C) (raw_init_clss S))
-     (removeAll_cond (\<lambda>D. mset (raw_clause D) = mset C) (raw_learned_clss S)) 
+     (removeAll_cond (\<lambda>D. mset (raw_clause D) = mset C) (raw_learned_clss S))
      (backtrack_lvl S)
      (raw_conflicting S)"
 
@@ -734,7 +734,7 @@ proof -
         apply fastforce
        using single_nil apply simp
       using single_other xs_def ys_def apply (metis list.set_intros(1) watch_nat_lists_disjointD)
-     using single_other unfolding xs_def ys_def apply (metis list.set_intros(1) 
+     using single_other unfolding xs_def ys_def apply (metis list.set_intros(1)
        watch_nat_lists_disjointD)
     using other xs_def ys_def by (metis H)+
 qed
@@ -840,7 +840,7 @@ next
         by simp
     next
       case (nil_single a)
-      moreover have "\<And>x. set C = {a} \<Longrightarrow> - a \<in> lits_of_l (trail S) \<Longrightarrow> x \<in> set (remove1 a C) \<Longrightarrow> 
+      moreover have "\<And>x. set C = {a} \<Longrightarrow> - a \<in> lits_of_l (trail S) \<Longrightarrow> x \<in> set (remove1 a C) \<Longrightarrow>
         x = a"
         using notin_set_remove1 by auto
       ultimately show ?thesis
@@ -852,7 +852,7 @@ next
     next
       case (single_nil a)
       show ?thesis
-        using watch_nat_lists_set_union_witness[of S C] 3 
+        using watch_nat_lists_set_union_witness[of S C] 3
         by (fastforce simp add: W ass tr single_nil comp_def distinct_filter_eq
           no_dup_distinct_map_uminus_lit_of min_def)
     next
@@ -1054,7 +1054,7 @@ next
           by (auto simp: distinct_mset_single_add)
       next
         case 2
-        have f2: "[l\<leftarrow>unwatched (TWL_Clause W UW) . l \<notin> set (watched (TWL_Clause W UW)) 
+        have f2: "[l\<leftarrow>unwatched (TWL_Clause W UW) . l \<notin> set (watched (TWL_Clause W UW))
           \<and> - l \<notin> insert (lit_of L) (lits_of_l (trail S))] \<noteq> []"
           using "2"(2) by simp
         then have "\<not> set UW \<subseteq> set W"
@@ -1063,7 +1063,7 @@ next
           using wf C "2"(1) by (auto simp: length_remove1)
       next
         case 3
-        have W: "length W \<le> Suc 0 \<longleftrightarrow> length W = 0 \<or> length W = Suc 0" 
+        have W: "length W \<le> Suc 0 \<longleftrightarrow> length W = 0 \<or> length W = Suc 0"
           by linarith
         show ?case
           using wf C 3 by (auto simp: length_remove1 W length_list_Suc_0 dest!: subset_singletonD)
@@ -1141,570 +1141,5 @@ interpretation twl2: abstract_twl watch_nat rewatch_nat "\<lambda>_. []"
   apply (rule clause_rewatch_witness'; simp add: image_image comp_def)
   apply (simp)
   done
-
-subsection \<open>Interpretation for @{term conflict_driven_clause_learning\<^sub>W.cdcl\<^sub>W}\<close>
-
-context abstract_twl
-begin
-
-subsubsection \<open>Direct Interpretation\<close>
-lemma mset_map_removeAll_cond:
-  "mset (map (\<lambda>x. mset (raw_clause x)) 
-    (removeAll_cond (\<lambda>D. mset (raw_clause D) = mset (raw_clause C)) N)) 
-  = mset (removeAll (mset (raw_clause C)) (map (\<lambda>x. mset (raw_clause x)) N))"
-  by (induction N) auto
-
-lemma mset_raw_init_clss_init_state:
-  "mset (map (\<lambda>x. mset (raw_clause x)) (raw_init_clss (init_state (map raw_clause N)))) 
-  = mset (map (\<lambda>x. mset (raw_clause x)) N)"
-  by (metis (no_types, lifting) init_clss_init_state map_eq_conv map_map o_def)
-
-interpretation rough_cdcl: state\<^sub>W 
-  "\<lambda>C. mset (raw_clause C)"
-    (* does not matter if the invariants do not hold *)
-  "\<lambda>L C. TWL_Clause (watched C) (L # unwatched C)"
-  "\<lambda>L C. TWL_Clause [] (remove1 L (watched C @ unwatched C))"
-  "\<lambda>C. clauses_of_l (map raw_clause C)" "op @"
-  "\<lambda>L C. L \<in> set C" "op #" "\<lambda>C. remove1_cond (\<lambda>D. mset (raw_clause D) = mset (raw_clause C))"
-
-  mset "\<lambda>xs ys. case_prod append (fold (\<lambda>x (ys, zs). (remove1 x ys, x # zs)) xs (ys, []))"
-  "op #" remove1
-
-  "\<lambda>C. watched C @ unwatched C" "\<lambda>C. TWL_Clause [] C"
-  trail "\<lambda>S. hd (raw_trail S)"
-  raw_init_clss raw_learned_clss backtrack_lvl raw_conflicting
-  cons_trail tl_trail "\<lambda>C. add_init_cls (raw_clause C)" "\<lambda>C. add_learned_cls (raw_clause C)" 
-  "\<lambda>C. remove_cls (raw_clause C)" 
-  update_backtrack_lvl
-  update_conflicting "\<lambda>N. init_state (map raw_clause N)" restart'
-  apply unfold_locales
-  apply (case_tac "raw_trail S")
-  apply (simp_all add: add_init_cls_def add_learned_cls_def clause_rewatch clause_watch
-    cons_trail_def remove_cls_def restart'_def tl_trail_def map_tl comp_def
-    ac_simps mset_map_removeAll_cond mset_raw_init_clss_init_state)
-  
-  apply (auto simp: mset_map image_mset_subseteq_mono[OF restart_learned] )
-  done
-
-interpretation rough_cdcl: conflict_driven_clause_learning\<^sub>W 
-  "\<lambda>C. mset (raw_clause C)"
-    (* does not matter if the invariants do not hold *)
-  "\<lambda>L C. TWL_Clause (watched C) (L # unwatched C)"
-  "\<lambda>L C. TWL_Clause [] (remove1 L (watched C @ unwatched C))"
-  "\<lambda>C. clauses_of_l (map raw_clause C)" "op @"
-  "\<lambda>L C. L \<in> set C" "op #" "\<lambda>C. remove1_cond (\<lambda>D. mset (raw_clause D) = mset (raw_clause C))"
-
-  mset "\<lambda>xs ys. case_prod append (fold (\<lambda>x (ys, zs). (remove1 x ys, x # zs)) xs (ys, []))"
-  "op #" remove1
-
-  "\<lambda>C. watched C @ unwatched C" "\<lambda>C. TWL_Clause [] C"
-  trail "\<lambda>S. hd (raw_trail S)"
-  raw_init_clss raw_learned_clss backtrack_lvl raw_conflicting
-  cons_trail tl_trail "\<lambda>C. add_init_cls (raw_clause C)" "\<lambda>C. add_learned_cls (raw_clause C)" 
-  "\<lambda>C. remove_cls (raw_clause C)" 
-  update_backtrack_lvl
-  update_conflicting "\<lambda>N. init_state (map raw_clause N)" restart'
-  by unfold_locales
-
-(* interpretation cdcl\<^sub>N\<^sub>O\<^sub>T: cdcl\<^sub>N\<^sub>O\<^sub>T_merge_bj_learn_ops
-  "\<lambda>S. convert_trail_from_W (trail S)"
-  rough_cdcl.clauses
-  "\<lambda>L S. cons_trail (convert_marked_lit_from_NOT L) S"
-  "\<lambda>S. tl_trail S"
-  "\<lambda>C S. add_learned_cls C S"
-  "\<lambda>C S. remove_cls C S"
-  (* propagate conditions: *)"\<lambda>L S. lit_of L \<in> fst ` candidates_propagate S"
-  "\<lambda>_ S. conflicting S = None"
-  "\<lambda>C C' L' S. C \<in> candidates_conflict S \<and> distinct_mset (C' + {#L'#}) \<and> \<not>tautology (C' + {#L'#})"
-  by unfold_locales
- *)
-subsubsection \<open>Opaque Type with Invariant\<close>
-
-declare rough_cdcl.state_simp[simp del]
-
-definition cons_trail_twl :: "('v, nat, 'v literal multiset) marked_lit \<Rightarrow> 'v wf_twl \<Rightarrow> 'v wf_twl"
-  where
-"cons_trail_twl L S \<equiv> twl_of_rough_state (cons_trail L (rough_state_of_twl S))"
-
-lemma wf_twl_state_cons_trail:
-  "undefined_lit (trail S) (lit_of L) \<Longrightarrow> wf_twl_state S \<Longrightarrow> wf_twl_state (cons_trail L S)"
-  unfolding wf_twl_state_def by (auto simp: cons_trail_def wf_rewatch defined_lit_map)
-
-lemma rough_state_of_twl_cons_trail:
-  "undefined_lit (trail_twl S) (lit_of L) \<Longrightarrow>
-    rough_state_of_twl (cons_trail_twl L S) = cons_trail L (rough_state_of_twl S)"
-  using rough_state_of_twl twl_of_rough_state_inverse wf_twl_state_cons_trail
-  unfolding cons_trail_twl_def by blast
-
-abbreviation add_init_cls_twl where
-"add_init_cls_twl C S \<equiv> twl_of_rough_state (add_init_cls C (rough_state_of_twl S))"
-
-lemma wf_twl_add_init_cls: "wf_twl_state S \<Longrightarrow> wf_twl_state (add_init_cls L S)"
-  unfolding wf_twl_state_def by (auto simp: wf_watch add_init_cls_def split: if_split_asm)
-
-lemma rough_state_of_twl_add_init_cls:
-  "rough_state_of_twl (add_init_cls_twl L S) = add_init_cls L (rough_state_of_twl S)"
-  using rough_state_of_twl twl_of_rough_state_inverse wf_twl_add_init_cls by blast
-
-abbreviation add_learned_cls_twl where
-"add_learned_cls_twl C S \<equiv> twl_of_rough_state (add_learned_cls C (rough_state_of_twl S))"
-
-lemma wf_twl_add_learned_cls: "wf_twl_state S \<Longrightarrow> wf_twl_state (add_learned_cls L S)"
-  unfolding wf_twl_state_def by (auto simp: wf_watch add_learned_cls_def split: if_split_asm)
-
-lemma rough_state_of_twl_add_learned_cls:
-  "rough_state_of_twl (add_learned_cls_twl L S) = add_learned_cls L (rough_state_of_twl S)"
-  using rough_state_of_twl twl_of_rough_state_inverse wf_twl_add_learned_cls by blast
-
-abbreviation remove_cls_twl where
-"remove_cls_twl C S \<equiv> twl_of_rough_state (remove_cls C (rough_state_of_twl S))"
-
-lemma wf_twl_remove_cls: "wf_twl_state S \<Longrightarrow> wf_twl_state (remove_cls L S)"
-  unfolding wf_twl_state_def by (auto simp: wf_watch remove_cls_def split: if_split_asm)
-
-lemma rough_state_of_twl_remove_cls:
-  "rough_state_of_twl (remove_cls_twl L S) = remove_cls L (rough_state_of_twl S)"
-  using rough_state_of_twl twl_of_rough_state_inverse wf_twl_remove_cls by blast
-
-abbreviation init_state_twl where
-"init_state_twl N \<equiv> twl_of_rough_state (init_state N)"
-
-lemma wf_twl_state_wf_twl_state_fold_add_init_cls:
-  assumes "wf_twl_state S"
-  shows "wf_twl_state (fold add_init_cls N S)"
-  using assms apply (induction N arbitrary: S)
-   apply (auto simp: wf_twl_state_def)[]
-  by (simp add: wf_twl_add_init_cls)
-
-lemma wf_twl_state_epsilon_state[simp]:
-  "wf_twl_state (TWL_State [] {#} {#} 0 None)"
-  by (auto simp: wf_twl_state_def)
-
-lemma wf_twl_init_state: "wf_twl_state (init_state N)"
-  unfolding init_state_def by (auto intro!: wf_twl_state_wf_twl_state_fold_add_init_cls)
-
-lemma rough_state_of_twl_init_state:
-  "rough_state_of_twl (init_state_twl N) = init_state N"
-  by (simp add: twl_of_rough_state_inverse wf_twl_init_state)
-
-abbreviation tl_trail_twl where
-"tl_trail_twl S \<equiv> twl_of_rough_state (tl_trail (rough_state_of_twl S))"
-
-lemma wf_twl_state_tl_trail: "wf_twl_state S \<Longrightarrow> wf_twl_state (tl_trail S)"
-  by (simp add: twl_of_rough_state_inverse wf_twl_init_state wf_twl_cls_wf_twl_cls_tl
-    tl_trail_def wf_twl_state_def distinct_tl map_tl)
-
-lemma rough_state_of_twl_tl_trail:
-  "rough_state_of_twl (tl_trail_twl S) = tl_trail (rough_state_of_twl S)"
-  using rough_state_of_twl twl_of_rough_state_inverse wf_twl_state_tl_trail by blast
-
-abbreviation update_backtrack_lvl_twl where
-"update_backtrack_lvl_twl k S \<equiv> twl_of_rough_state (update_backtrack_lvl k (rough_state_of_twl S))"
-
-lemma wf_twl_state_update_backtrack_lvl:
-  "wf_twl_state S \<Longrightarrow> wf_twl_state (update_backtrack_lvl k S)"
-  unfolding wf_twl_state_def by auto
-
-lemma rough_state_of_twl_update_backtrack_lvl:
-  "rough_state_of_twl (update_backtrack_lvl_twl k S) = update_backtrack_lvl k
-    (rough_state_of_twl S)"
-  using rough_state_of_twl twl_of_rough_state_inverse wf_twl_state_update_backtrack_lvl by fast
-
-abbreviation update_conflicting_twl where
-"update_conflicting_twl k S \<equiv> twl_of_rough_state (update_conflicting k (rough_state_of_twl S))"
-
-lemma wf_twl_state_update_conflicting:
-  "wf_twl_state S \<Longrightarrow> wf_twl_state (update_conflicting k S)"
-  unfolding wf_twl_state_def by auto
-
-lemma rough_state_of_twl_update_conflicting:
-  "rough_state_of_twl (update_conflicting_twl k S) = update_conflicting k
-    (rough_state_of_twl S)"
-  using rough_state_of_twl twl_of_rough_state_inverse wf_twl_state_update_conflicting by fast
-
-abbreviation raw_clauses_twl where
-"raw_clauses_twl S \<equiv> raw_clauses (rough_state_of_twl S)"
-
-abbreviation restart_twl where
-"restart_twl S \<equiv> twl_of_rough_state (restart' (rough_state_of_twl S))"
-
-lemma wf_wf_restart': "wf_twl_state S \<Longrightarrow> wf_twl_state (restart' S)"
-  unfolding restart'_def wf_twl_state_def apply standard
-   apply clarify
-   apply (rename_tac x)
-   apply (subgoal_tac "wf_twl_cls (trail S) x")
-    apply (case_tac x)
-  using restart_learned by fastforce+
-
-lemma rough_state_of_twl_restart_twl:
-  "rough_state_of_twl (restart_twl S) = restart' (rough_state_of_twl S)"
-  by (simp add: twl_of_rough_state_inverse wf_wf_restart')
-
-(* Sledgehammer is awesome! *)
-interpretation cdcl\<^sub>W_twl_NOT: dpll_state
-  "\<lambda>S. convert_trail_from_W (trail_twl S)"
-  raw_clauses_twl
-  "\<lambda>L S. cons_trail_twl (convert_marked_lit_from_NOT L) S"
-  "\<lambda>S. tl_trail_twl S"
-  "\<lambda>C S. add_learned_cls_twl C S"
-  "\<lambda>C S. remove_cls_twl C S"
-  apply unfold_locales
-         apply (simp add: rough_state_of_twl_cons_trail)
-        apply (metis rough_state_of_twl_tl_trail rough_cdcl.tl_trail)
-       apply (metis rough_state_of_twl_add_learned_cls rough_cdcl.trail_add_cls\<^sub>N\<^sub>O\<^sub>T)
-      apply (metis rough_state_of_twl_remove_cls rough_cdcl.trail_remove_cls)
-     apply (simp add: rough_state_of_twl_cons_trail)
-    apply (simp add: rough_state_of_twl_tl_trail)
-   using rough_cdcl.clauses_add_cls\<^sub>N\<^sub>O\<^sub>T rough_cdcl.clauses_def rough_state_of_twl_add_learned_cls
-   apply auto[1]
-  using rough_cdcl.clauses_def rough_cdcl.clauses_remove_cls rough_state_of_twl_remove_cls by auto
-
-interpretation cdcl\<^sub>W_twl: state\<^sub>W
-  trail_twl
-  init_clss_twl
-  learned_clss_twl
-  backtrack_lvl_twl
-  conflicting_twl
-  cons_trail_twl
-  tl_trail_twl
-  add_init_cls_twl
-  add_learned_cls_twl
-  remove_cls_twl
-  update_backtrack_lvl_twl
-  update_conflicting_twl
-  init_state_twl
-  restart_twl
-  apply unfold_locales
-  by (simp_all add: rough_state_of_twl_cons_trail rough_state_of_twl_tl_trail
-    rough_state_of_twl_add_init_cls rough_state_of_twl_add_learned_cls rough_state_of_twl_remove_cls
-    rough_state_of_twl_update_backtrack_lvl rough_state_of_twl_update_conflicting
-    rough_state_of_twl_init_state rough_state_of_twl_restart_twl
-    rough_cdcl.learned_clss_restart_state)
-
-interpretation cdcl\<^sub>W_twl: cdcl\<^sub>W
-  trail_twl
-  init_clss_twl
-  learned_clss_twl
-  backtrack_lvl_twl
-  conflicting_twl
-  cons_trail_twl
-  tl_trail_twl
-  add_init_cls_twl
-  add_learned_cls_twl
-  remove_cls_twl
-  update_backtrack_lvl_twl
-  update_conflicting_twl
-  init_state_twl
-  restart_twl
-  by unfold_locales
-
-sublocale cdcl\<^sub>W
-  trail_twl
-  init_clss_twl
-  learned_clss_twl
-  backtrack_lvl_twl
-  conflicting_twl
-  cons_trail_twl
-  tl_trail_twl
-  add_init_cls_twl
-  add_learned_cls_twl
-  remove_cls_twl
-  update_backtrack_lvl_twl
-  update_conflicting_twl
-  init_state_twl
-  restart_twl
-  by (rule cdcl\<^sub>W_twl.cdcl\<^sub>W_axioms)
-
-abbreviation state_eq_twl (infix "\<sim>TWL" 51) where
-"state_eq_twl S S' \<equiv> rough_cdcl.state_eq (rough_state_of_twl S) (rough_state_of_twl S')"
-notation cdcl\<^sub>W_twl.state_eq (infix "\<sim>" 51)
-declare cdcl\<^sub>W_twl.state_simp[simp del]
-  cdcl\<^sub>W_twl_NOT.state_simp\<^sub>N\<^sub>O\<^sub>T[simp del]
-
-text \<open>To avoid ambiguities:\<close>
-no_notation state_eq_twl (infix "\<sim>" 51)
-
-definition propagate_twl where
-"propagate_twl S S' \<longleftrightarrow>
-  (\<exists>L C. (L, C) \<in> candidates_propagate_twl S
-  \<and> S' \<sim> cons_trail_twl (Propagated L C) S
-  \<and> conflicting_twl S = None)"
-
-lemma propagate_twl_iff_propagate:
-  assumes inv: "cdcl\<^sub>W_twl.cdcl\<^sub>W_all_struct_inv S"
-  shows "cdcl\<^sub>W_twl.propagate S T \<longleftrightarrow> propagate_twl S T" (is "?P \<longleftrightarrow> ?T")
-proof
-  assume ?P
-  then obtain C L where
-    "conflicting (rough_state_of_twl S) = None" and
-    CL_Clauses: "C + {#L#} \<in># cdcl\<^sub>W_twl.clauses S" and
-    tr_CNot: "trail_twl S \<Turnstile>as CNot C" and
-    undef_lot: "undefined_lit (trail_twl S) L" and
-    "T \<sim> cons_trail_twl (Propagated L (C + {#L#})) S"
-    unfolding cdcl\<^sub>W_twl.propagate.simps by blast
-  have "distinct_mset (C + {#L#})"
-    using inv CL_Clauses unfolding cdcl\<^sub>W_twl.cdcl\<^sub>W_all_struct_inv_def
-    cdcl\<^sub>W_twl.distinct_cdcl\<^sub>W_state_def cdcl\<^sub>W_twl.clauses_def distinct_mset_set_def
-    by auto
-  then have C_L_L: "mset_set (set_mset (C + {#L#}) - {L}) = C"
-    by (metis Un_insert_right add_diff_cancel_left' add_diff_cancel_right'
-      distinct_mset_set_mset_ident finite_set_mset insert_absorb2 mset_set.insert_remove
-      set_mset_single set_mset_union)
-  have "(L, C+{#L#}) \<in> candidates_propagate_twl S"
-    apply (rule wf_candidates_propagate_complete)
-         using rough_state_of_twl apply auto[]
-        using CL_Clauses unfolding cdcl\<^sub>W_twl.clauses_def apply auto[]
-       apply simp
-      using C_L_L tr_CNot apply simp
-     using undef_lot apply blast
-     done
-  show ?T unfolding propagate_twl_def
-    apply (rule exI[of _ "L"], rule exI[of _ "C+{#L#}"])
-    apply (auto simp: \<open>(L, C+{#L#}) \<in> candidates_propagate_twl S\<close>
-      \<open>conflicting (rough_state_of_twl S) = None\<close> )
-    using \<open>T \<sim> cons_trail_twl (Propagated L (C + {#L#})) S\<close> cdcl\<^sub>W_twl.state_eq_backtrack_lvl
-    cdcl\<^sub>W_twl.state_eq_conflicting cdcl\<^sub>W_twl.state_eq_init_clss
-    cdcl\<^sub>W_twl.state_eq_learned_clss cdcl\<^sub>W_twl.state_eq_trail rough_cdcl.state_eq_def by blast
-next
-  assume ?T
-  then obtain L C where
-    LC: "(L, C) \<in> candidates_propagate_twl S" and
-    T: "T \<sim> cons_trail_twl (Propagated L C) S" and
-    confl: "conflicting (rough_state_of_twl S) = None"
-    unfolding propagate_twl_def by auto
-  have [simp]: "C - {#L#} + {#L#} = C"
-    using LC unfolding candidates_propagate_def
-    by clarify (metis Multiset.diff_le_self insert_DiffM2 mset_leD multi_member_last union_iff)
-  have "C \<in># raw_clauses_twl S"
-    using LC unfolding candidates_propagate_def rough_cdcl.clauses_def by auto
-  then have "distinct_mset C"
-    using inv unfolding cdcl\<^sub>W_twl.cdcl\<^sub>W_all_struct_inv_def cdcl\<^sub>W_twl.distinct_cdcl\<^sub>W_state_def
-    cdcl\<^sub>W_twl.clauses_def distinct_mset_set_def rough_cdcl.clauses_def by auto
-  then have C_L_L: "mset_set (set_mset C - {L}) = C - {#L#}"
-    by (metis \<open>C - {#L#} + {#L#} = C\<close> add_left_imp_eq diff_single_trivial
-      distinct_mset_set_mset_ident finite_set_mset mset_set.remove
-      multi_self_add_other_not_self union_commute)
-
-  show ?P
-    apply (rule cdcl\<^sub>W_twl.propagate.intros[of _ "trail_twl S" "init_clss_twl S"
-      "learned_clss_twl S" "backtrack_lvl_twl S" "C-{#L#}" L])
-        using confl apply auto[]
-       using LC unfolding candidates_propagate_def apply (auto simp: cdcl\<^sub>W_twl.clauses_def)[]
-      using wf_candidates_propagate_sound[OF _ LC] rough_state_of_twl apply (simp add: C_L_L)
-     using wf_candidates_propagate_sound[OF _ LC] rough_state_of_twl apply simp
-    using T unfolding cdcl\<^sub>W_twl.state_eq_def rough_cdcl.state_eq_def by auto
-qed
-no_notation CDCL_Two_Watched_Literals.twl.state_eq_twl (infix "\<sim>TWL" 51)
-definition conflict_twl where
-"conflict_twl S S' \<longleftrightarrow>
-  (\<exists>C. C \<in> candidates_conflict_twl S
-  \<and> S' \<sim> update_conflicting_twl (Some C) S
-  \<and> conflicting_twl S = None)"
-
-lemma conflict_twl_iff_conflict:
-  shows "cdcl\<^sub>W_twl.conflict S T \<longleftrightarrow> conflict_twl S T" (is "?C \<longleftrightarrow> ?T")
-proof
-  assume ?C
-  then obtain M N U k C where
-    S: "rough_cdcl.state (rough_state_of_twl S) = (M, N, U, k, None)" and
-    C: "C \<in># cdcl\<^sub>W_twl.clauses S" and
-    M_C: "M \<Turnstile>as CNot C" and
-    T: "T \<sim> update_conflicting_twl (Some C) S"
-    by auto
-  have "C \<in> candidates_conflict_twl S"
-    apply (rule wf_candidates_conflict_complete)
-       apply simp
-      using C apply (auto simp: cdcl\<^sub>W_twl.clauses_def)[]
-    using M_C S by auto
-  moreover have "T \<sim> twl_of_rough_state (update_conflicting (Some C) (rough_state_of_twl S))"
-    using T unfolding rough_cdcl.state_eq_def cdcl\<^sub>W_twl.state_eq_def by auto
-  ultimately show ?T
-    using S unfolding conflict_twl_def by auto
-next
-  assume ?T
-  then obtain C where
-    C: "C \<in> candidates_conflict_twl S" and
-    T: "T \<sim> update_conflicting_twl (Some C) S" and
-    confl: "conflicting_twl S = None"
-    unfolding conflict_twl_def by auto
-  have "C \<in># cdcl\<^sub>W_twl.clauses S"
-    using C unfolding candidates_conflict_def cdcl\<^sub>W_twl.clauses_def by auto
- moreover have "trail_twl S \<Turnstile>as CNot C"
-    using wf_candidates_conflict_sound[OF _ C] by auto
- ultimately show ?C apply -
-   apply (rule cdcl\<^sub>W_twl.conflict.conflict_rule[of _ _ _ _ _ C])
-   using confl T unfolding rough_cdcl.state_eq_def cdcl\<^sub>W_twl.state_eq_def by auto
-qed
-
-inductive cdcl\<^sub>W_twl :: "'v wf_twl \<Rightarrow> 'v wf_twl \<Rightarrow> bool" for S :: "'v wf_twl" where
-propagate: "propagate_twl S S' \<Longrightarrow> cdcl\<^sub>W_twl S S'" |
-conflict: "conflict_twl S S' \<Longrightarrow> cdcl\<^sub>W_twl S S'" |
-other: "cdcl\<^sub>W_twl.cdcl\<^sub>W_o S S' \<Longrightarrow> cdcl\<^sub>W_twl S S'"|
-rf: "cdcl\<^sub>W_twl.cdcl\<^sub>W_rf S S' \<Longrightarrow> cdcl\<^sub>W_twl S S'"
-
-lemma cdcl\<^sub>W_twl_iff_cdcl\<^sub>W:
-  assumes "cdcl\<^sub>W_twl.cdcl\<^sub>W_all_struct_inv S"
-  shows "cdcl\<^sub>W_twl S T \<longleftrightarrow> cdcl\<^sub>W_twl.cdcl\<^sub>W S T"
-  by (simp add: assms cdcl\<^sub>W_twl.cdcl\<^sub>W.simps cdcl\<^sub>W_twl.simps conflict_twl_iff_conflict
-    propagate_twl_iff_propagate)
-
-lemma rtranclp_cdcl\<^sub>W_twl_all_struct_inv_inv:
-  assumes "cdcl\<^sub>W_twl\<^sup>*\<^sup>* S T" and "cdcl\<^sub>W_twl.cdcl\<^sub>W_all_struct_inv S"
-  shows "cdcl\<^sub>W_twl.cdcl\<^sub>W_all_struct_inv T"
-  using assms by (induction rule: rtranclp_induct)
-  (simp_all add: cdcl\<^sub>W_twl_iff_cdcl\<^sub>W cdcl\<^sub>W_twl.cdcl\<^sub>W_all_struct_inv_inv)
-
-lemma rtranclp_cdcl\<^sub>W_twl_iff_rtranclp_cdcl\<^sub>W:
-  assumes "cdcl\<^sub>W_twl.cdcl\<^sub>W_all_struct_inv S"
-  shows "cdcl\<^sub>W_twl\<^sup>*\<^sup>* S T \<longleftrightarrow> cdcl\<^sub>W_twl.cdcl\<^sub>W\<^sup>*\<^sup>* S T" (is "?T \<longleftrightarrow> ?W")
-proof
-  assume ?W
-  then show ?T
-    proof (induction rule: rtranclp_induct)
-      case base
-      then show ?case by simp
-    next
-      case (step T U) note st = this(1) and cdcl = this(2) and IH = this(3)
-      have "cdcl\<^sub>W_twl T U"
-        using assms st cdcl cdcl\<^sub>W_twl.rtranclp_cdcl\<^sub>W_all_struct_inv_inv cdcl\<^sub>W_twl_iff_cdcl\<^sub>W
-        by blast
-      then show ?case using IH by auto
-    qed
-next
-  assume ?T
-  then show ?W
-    proof (induction rule: rtranclp_induct)
-      case base
-      then show ?case by simp
-    next
-      case (step T U) note st = this(1) and cdcl = this(2) and IH = this(3)
-      have "cdcl\<^sub>W_twl.cdcl\<^sub>W T U"
-        using assms st cdcl rtranclp_cdcl\<^sub>W_twl_all_struct_inv_inv cdcl\<^sub>W_twl_iff_cdcl\<^sub>W
-        by blast
-      then show ?case using IH by auto
-    qed
-qed
-
-interpretation cdcl\<^sub>N\<^sub>O\<^sub>T_twl: backjumping_ops
-  "\<lambda>S. convert_trail_from_W (trail_twl S)"
-  abstract_twl.raw_clauses_twl
-  "\<lambda>L (S:: 'v wf_twl).
-    cons_trail_twl
-      (convert_marked_lit_from_NOT L) (S:: 'v wf_twl)"
-  tl_trail_twl
-  add_learned_cls_twl
-  remove_cls_twl
-  (* bj conditions *) "\<lambda>C _ _ (S:: 'v wf_twl) _. C \<in> candidates_conflict_twl S"
-  by unfold_locales
-
-lemma reduce_trail_to\<^sub>N\<^sub>O\<^sub>T_skip_beginning_twl:
-  assumes "trail_twl S = convert_trail_from_NOT (F' @ F)"
-  shows "trail_twl (cdcl\<^sub>W_twl.reduce_trail_to\<^sub>N\<^sub>O\<^sub>T F S) = convert_trail_from_NOT F"
-  using assms by (induction F' arbitrary: S) auto
-
-lemma reduce_trail_to\<^sub>N\<^sub>O\<^sub>T_trail_tl_trail_twl_decomp[simp]:
-  "trail_twl S = convert_trail_from_NOT (F' @ Marked K () # F) \<Longrightarrow>
-     trail_twl (cdcl\<^sub>W_twl.reduce_trail_to\<^sub>N\<^sub>O\<^sub>T F (tl_trail_twl S)) = convert_trail_from_NOT F"
-  apply (rule reduce_trail_to\<^sub>N\<^sub>O\<^sub>T_skip_beginning_twl[of _ "tl (F' @ Marked K () # [])"])
-  by (cases F') (auto simp add:tl_append rough_cdcl.reduce_trail_to\<^sub>N\<^sub>O\<^sub>T_skip_beginning)
-
-lemma trail_twl_reduce_trail_to\<^sub>N\<^sub>O\<^sub>T_drop:
-  "trail_twl (cdcl\<^sub>W_twl.reduce_trail_to\<^sub>N\<^sub>O\<^sub>T F S) =
-    (if length (trail_twl S) \<ge> length F
-    then drop (length (trail_twl S) - length F) (trail_twl S)
-    else [])"
-  apply (induction F S rule: cdcl\<^sub>W_twl.reduce_trail_to\<^sub>N\<^sub>O\<^sub>T.induct)
-  apply (rename_tac F S)
-  apply (case_tac "trail_twl S")
-   apply auto[]
-  apply (rename_tac list)
-  apply (case_tac "Suc (length list) > length F")
-   prefer 2 apply simp
-  apply (subgoal_tac "Suc (length list) - length F = Suc (length list - length F)")
-   apply simp
-  apply simp
-  done
-
-interpretation cdcl\<^sub>N\<^sub>O\<^sub>T_twl: dpll_with_backjumping_ops
-  "\<lambda>S. convert_trail_from_W (trail_twl S)"
-  abstract_twl.raw_clauses_twl
-  "\<lambda>L S.
-    cons_trail_twl
-      (convert_marked_lit_from_NOT L) S"
-  tl_trail_twl
-  add_learned_cls_twl
-  remove_cls_twl
-  (* propagate conditions: *)"\<lambda>L S. lit_of L \<in> fst ` candidates_propagate_twl S"
-  (* state invariant *)"\<lambda>S. no_dup (trail_twl S)"
-  (* backjump conditions *)"\<lambda>C _ _ S _. C \<in> candidates_conflict_twl S"
-proof (unfold_locales, goal_cases)
-  case (1 C' S C F' K F L) note n_d = this(1) and n_d' = this(2) and undef = this(6)
-  let ?T' = "(cons_trail (Propagated L {#}) (rough_state_of_twl (cdcl\<^sub>W_twl.reduce_trail_to\<^sub>N\<^sub>O\<^sub>T F S)))"
-  let ?T = "(cons_trail_twl (Propagated L {#}) (cdcl\<^sub>W_twl.reduce_trail_to\<^sub>N\<^sub>O\<^sub>T F S))"
-  have tr_F_S: "map lit_of (trail_twl (cdcl\<^sub>W_twl.reduce_trail_to\<^sub>N\<^sub>O\<^sub>T F S)) =
-    map lit_of (convert_trail_from_NOT F)"
-    apply (subst trail_twl_reduce_trail_to\<^sub>N\<^sub>O\<^sub>T_drop[of F S])
-    using 1(1) arg_cong[OF 1(3), of length] arg_cong[OF 1(3), of "map lit_of"]
-    by (auto simp: o_def drop_map[symmetric])
-
-  have "no_dup (trail_twl S)"
-    using "1"(1) by blast
-  have "wf_twl_state (rough_state_of_twl (cdcl\<^sub>W_twl.reduce_trail_to\<^sub>N\<^sub>O\<^sub>T F S))"
-    using wf_twl_state_rough_state_of_twl by blast
-  moreover have undef': "undefined_lit (trail_twl (cdcl\<^sub>W_twl.reduce_trail_to\<^sub>N\<^sub>O\<^sub>T F S)) L"
-    using undef arg_cong[OF tr_F_S, of "map atm_of"] unfolding defined_lit_map image_set
-    by (simp add:  o_def)
-  ultimately have "wf_twl_state ?T'"
-    by (simp_all add: wf_twl_state_cons_trail)
-  then have "init_clss_twl ?T = init_clss_twl (cdcl\<^sub>W_twl.reduce_trail_to\<^sub>N\<^sub>O\<^sub>T F S)"
-      using 1(6) by (simp add: undef')
-  then have [simp]: "init_clss_twl ?T = init_clss_twl S"
-     by (simp add: cdcl\<^sub>W_twl.reduce_trail_to\<^sub>N\<^sub>O\<^sub>T_reduce_trail_convert)
-
-  have "learned_clss_twl ?T = learned_clss_twl (cdcl\<^sub>W_twl.reduce_trail_to\<^sub>N\<^sub>O\<^sub>T F S)"
-    by (smt "1"(3) "1"(6) append_assoc cdcl\<^sub>W_twl.learned_clss_cons_trail
-      cdcl\<^sub>W_twl_NOT.reduce_trail_to\<^sub>N\<^sub>O\<^sub>T_eq_length cdcl\<^sub>W_twl_NOT.reduce_trail_to\<^sub>N\<^sub>O\<^sub>T_nil
-      cdcl\<^sub>W_twl_NOT.reduce_trail_to\<^sub>N\<^sub>O\<^sub>T_skip_beginning comp_apply defined_lit_convert_trail_from_W
-      list.sel(3) marked_lit.sel(2) rev.simps(2) rev_append rev_eq_Cons_iff
-      cons_trail_twl_def)
-  moreover have "learned_clss_twl (cdcl\<^sub>W_twl.reduce_trail_to\<^sub>N\<^sub>O\<^sub>T F S)
-    = learned_clss_twl S"
-    by (simp add: cdcl\<^sub>W_twl.reduce_trail_to\<^sub>N\<^sub>O\<^sub>T_reduce_trail_convert)
-  ultimately have [simp]: "learned_clss_twl ?T = learned_clss_twl S"
-    by simp
-  have tr_L_F_S: "map lit_of (trail_twl ?T)
-    = map lit_of (Propagated L {#} # convert_trail_from_NOT F)"
-    using undef' tr_F_S by (simp add: o_def)
-  have C_confl_cand: "C \<in> candidates_conflict_twl S"
-    apply(rule wf_candidates_twl_conflict_complete)
-     using 1(1,4) apply (simp add: rough_cdcl.clauses_def)
-    using 1(5) by (simp add: tr_L_F_S true_annots_true_cls lits_of_l_convert_trail_from_NOT)
-
-  have "cdcl\<^sub>N\<^sub>O\<^sub>T_twl.backjump S
-    (cons_trail_twl (convert_marked_lit_from_NOT (Propagated L ()))
-      (cdcl\<^sub>W_twl.reduce_trail_to\<^sub>N\<^sub>O\<^sub>T F S))"
-    apply (rule cdcl\<^sub>N\<^sub>O\<^sub>T_twl.backjump.intros[of S F' K F _ L C, OF 1(3) _ 1(4-6) _ 1(8-9)])
-      unfolding cdcl\<^sub>W_twl_NOT.state_eq\<^sub>N\<^sub>O\<^sub>T_def apply (metis convert_marked_lit_from_NOT.simps(1))
-     using 1(7) 1(3) apply presburger
-    using C_confl_cand by simp
-  then show ?case
-    by blast
-qed
-
-interpretation cdcl\<^sub>N\<^sub>O\<^sub>T_twl: dpll_with_backjumping
-  "\<lambda>S. convert_trail_from_W (trail_twl S)"
-  abstract_twl.raw_clauses_twl
-  "\<lambda>L (S:: 'v wf_twl).
-    cons_trail_twl
-      (convert_marked_lit_from_NOT L) (S:: 'v wf_twl)"
-  tl_trail_twl
-  add_learned_cls_twl
-  remove_cls_twl
-  (* propagate conditions: *)"\<lambda>L S. lit_of L \<in> fst ` candidates_propagate_twl S"
-  (* state invariant *)"\<lambda>S. no_dup (trail_twl S)"
-  (* backjump conditions *)"\<lambda>C _ _ (S:: 'v wf_twl) _. C \<in> candidates_conflict_twl S"
-  apply unfold_locales
-  using cdcl\<^sub>N\<^sub>O\<^sub>T_twl.dpll_bj_no_dup by (simp add: o_def)
-end
 
 end
