Weidenbach_Book/CDCL_Two_Watched_Literals_Implementation.thy
@@ -8,295 +8,572 @@ theory CDCL_Two_Watched_Literals_Implementation
 imports CDCL_Two_Watched_Literals DPLL_CDCL_W_Implementation
 begin
 
-type_synonym 'v conc_twl_state =
-  "(('v, nat, 'v literal list) marked_lit, 'v literal list twl_clause list, nat, 'v literal list)
-    twl_state"
+subsection \<open>Interpretation for @{term conflict_driven_clause_learning\<^sub>W.cdcl\<^sub>W}\<close>
 
-fun convert :: "('a, 'b, 'c list) marked_lit \<Rightarrow> ('a, 'b, 'c multiset) marked_lit"  where
-"convert (Propagated L C) = Propagated L (mset C)" |
-"convert (Marked K i) = Marked K i"
+context abstract_twl
+begin
 
-abbreviation convert_tr :: "('a, 'b, 'c list) marked_lits \<Rightarrow> ('a, 'b, 'c multiset) marked_lits"
-  where
-"convert_tr \<equiv> map convert"
+subsubsection \<open>Direct Interpretation\<close>
+lemma mset_map_removeAll_cond:
+  "mset (map (\<lambda>x. mset (raw_clause x))
+    (removeAll_cond (\<lambda>D. mset (raw_clause D) = mset (raw_clause C)) N))
+  = mset (removeAll (mset (raw_clause C)) (map (\<lambda>x. mset (raw_clause x)) N))"
+  by (induction N) auto
 
-abbreviation convertC :: "'a literal list option \<Rightarrow> 'a clause option"  where
-"convertC \<equiv> map_option mset"
+lemma mset_raw_init_clss_init_state:
+  "mset (map (\<lambda>x. mset (raw_clause x)) (raw_init_clss (init_state (map raw_clause N))))
+  = mset (map (\<lambda>x. mset (raw_clause x)) N)"
+  by (metis (no_types, lifting) init_clss_init_state map_eq_conv map_map o_def)
 
-fun raw_clause_l :: "'v list twl_clause \<Rightarrow> 'v multiset twl_clause"  where
-  "raw_clause_l (TWL_Clause UW W) = TWL_Clause (mset W) (mset UW)"
+interpretation rough_cdcl: state\<^sub>W
+  "\<lambda>C. mset (raw_clause C)"
+    (* does not matter if the invariants do not hold *)
+  "\<lambda>L C. TWL_Clause (watched C) (L # unwatched C)"
+  "\<lambda>L C. TWL_Clause [] (remove1 L (watched C @ unwatched C))"
+  "\<lambda>C. clauses_of_l (map raw_clause C)" "op @"
+  "\<lambda>L C. L \<in> set C" "op #" "\<lambda>C. remove1_cond (\<lambda>D. mset (raw_clause D) = mset (raw_clause C))"
 
-abbreviation convert_clss :: "'v literal list twl_clause list \<Rightarrow> 'v clause twl_clause multiset"
-  where
-"convert_clss S \<equiv> mset (map raw_clause_l S)"
+  mset "\<lambda>xs ys. case_prod append (fold (\<lambda>x (ys, zs). (remove1 x ys, x # zs)) xs (ys, []))"
+  "op #" remove1
 
-fun raw_state_of_conc :: "'v conc_twl_state \<Rightarrow> ('v, nat, 'v clause) twl_state_abs" where
-"raw_state_of_conc (TWL_State M N U k C) =
-  TWL_State (convert_tr M) (convert_clss N) (convert_clss U) k (map_option mset C)"
+  "\<lambda>C. watched C @ unwatched C" "\<lambda>C. TWL_Clause [] C"
+  trail "\<lambda>S. hd (raw_trail S)"
+  raw_init_clss raw_learned_clss backtrack_lvl raw_conflicting
+  cons_trail tl_trail "\<lambda>C. add_init_cls (raw_clause C)" "\<lambda>C. add_learned_cls (raw_clause C)"
+  "\<lambda>C. remove_cls (raw_clause C)"
+  update_backtrack_lvl
+  update_conflicting "\<lambda>N. init_state (map raw_clause N)" restart'
+  apply unfold_locales
+  apply (case_tac "raw_trail S")
+  apply (simp_all add: add_init_cls_def add_learned_cls_def clause_rewatch clause_watch
+    cons_trail_def remove_cls_def restart'_def tl_trail_def map_tl comp_def
+    ac_simps mset_map_removeAll_cond mset_raw_init_clss_init_state)
 
-lemma
-  "raw_state_of_conc (tl_trail S) = tl_trail (raw_state_of_conc S)"
-  unfolding tl_trail_def by (induction S) (auto simp: map_tl)
+  apply (auto simp: mset_map image_mset_subseteq_mono[OF restart_learned] )
+  done
 
-typedef 'v conv_twl_state = "{S:: 'v conc_twl_state. wf_twl_state (raw_state_of_conc S)}"
-morphisms list_twl_state_of cls_twl_state
-proof -
-    have "TWL_State [] [] [] 0 None \<in> {S:: 'v conc_twl_state. wf_twl_state (raw_state_of_conc S)}"
-      by (auto simp: wf_twl_state_def)
-    then show ?thesis by blast
-qed
-term list_twl_state_of
+interpretation rough_cdcl: conflict_driven_clause_learning\<^sub>W
+  "\<lambda>C. mset (raw_clause C)"
+    (* does not matter if the invariants do not hold *)
+  "\<lambda>L C. TWL_Clause (watched C) (L # unwatched C)"
+  "\<lambda>L C. TWL_Clause [] (remove1 L (watched C @ unwatched C))"
+  "\<lambda>C. clauses_of_l (map raw_clause C)" "op @"
+  "\<lambda>L C. L \<in> set C" "op #" "\<lambda>C. remove1_cond (\<lambda>D. mset (raw_clause D) = mset (raw_clause C))"
 
-definition watch_list :: "'v conv_twl_state \<Rightarrow> 'v literal list \<Rightarrow> 'v literal list twl_clause" where
-  "watch_list S' C =
-   (let
-      M = trail (list_twl_state_of S');
-      C' = remdups C;
-      negation_not_assigned = filter (\<lambda>L. -L \<notin> lits_of M) C';
-      negation_assigned_sorted_by_trail = filter (\<lambda>L. L \<in> set C) (map (\<lambda>L. -lit_of L) M);
-      W = take 2 (negation_not_assigned @ negation_assigned_sorted_by_trail);
-      UW = foldl (\<lambda>a l. remove1 l a) C W
-    in TWL_Clause W UW)"
+  mset "\<lambda>xs ys. case_prod append (fold (\<lambda>x (ys, zs). (remove1 x ys, x # zs)) xs (ys, []))"
+  "op #" remove1
 
-lemma wf_watch_nat: "no_dup (trail (list_twl_state_of S)) \<Longrightarrow>
-  wf_twl_cls (trail (list_twl_state_of S)) (raw_clause_l (watch_list S C))"
-  apply (simp only: watch_list_def Let_def raw_clause_l.simps)
-  using wf_watch_witness[of "(list_twl_state_of S)" "C" "mset C"]
-oops
-(*
-definition
-  rewatch_nat ::
-  "(nat, nat, nat literal list) marked_lit \<Rightarrow> conc_twl_state \<Rightarrow>
-    nat literal list twl_clause \<Rightarrow> nat literal list twl_clause"
-where
-  "rewatch_nat L S C =
-   (if - lit_of L \<in> set (watched C) then
-      case filter (\<lambda>L'. L' \<notin> set (watched C) \<and> - L' \<notin> lits_of (L # trail S))
-          (unwatched C) of
-        [] \<Rightarrow> C
-      | L' # _ \<Rightarrow>
-        TWL_Clause (L' # remove1 (- lit_of L) (watched C))
-          (- lit_of L # remove1 L' (unwatched C))
-    else
-      C)"
+  "\<lambda>C. watched C @ unwatched C" "\<lambda>C. TWL_Clause [] C"
+  trail "\<lambda>S. hd (raw_trail S)"
+  raw_init_clss raw_learned_clss backtrack_lvl raw_conflicting
+  cons_trail tl_trail "\<lambda>C. add_init_cls (raw_clause C)" "\<lambda>C. add_learned_cls (raw_clause C)"
+  "\<lambda>C. remove_cls (raw_clause C)"
+  update_backtrack_lvl
+  update_conflicting "\<lambda>N. init_state (map raw_clause N)" restart'
+  by unfold_locales
 
-definition raw_candidates_conflict :: "conc_twl_state \<Rightarrow> nat literal list list" where
-  "raw_candidates_conflict S =
-    map (\<lambda>T. case T of TWL_Clause W UW \<Rightarrow> W @ UW)
-       (filter (\<lambda>C. set (watched C) \<subseteq> (uminus ` lits_of (trail S)))
-       (init_clss S @ learned_clss S))"
-
-definition do_conflict_step :: "conc_twl_state \<Rightarrow> conc_twl_state option" where
-"do_conflict_step S =
-  (case conflicting S of
-    Some _ \<Rightarrow> None
-  | None \<Rightarrow>
-      (case raw_candidates_conflict S of
-        [] \<Rightarrow> None
-      | a # _ \<Rightarrow> Some (update_conflicting (Some a) S)))"
+(* interpretation cdcl\<^sub>N\<^sub>O\<^sub>T: cdcl\<^sub>N\<^sub>O\<^sub>T_merge_bj_learn_ops
+  "\<lambda>S. convert_trail_from_W (trail S)"
+  rough_cdcl.clauses
+  "\<lambda>L S. cons_trail (convert_marked_lit_from_NOT L) S"
+  "\<lambda>S. tl_trail S"
+  "\<lambda>C S. add_learned_cls C S"
+  "\<lambda>C S. remove_cls C S"
+  (* propagate conditions: *)"\<lambda>L S. lit_of L \<in> fst ` candidates_propagate S"
+  "\<lambda>_ S. conflicting S = None"
+  "\<lambda>C C' L' S. C \<in> candidates_conflict S \<and> distinct_mset (C' + {#L'#}) \<and> \<not>tautology (C' + {#L'#})"
+  by unfold_locales
  *)
-(*
-lemma do_conflict_step_Some:
-  assumes conf: "do_conflict_step S = Some T"
-  shows "twl.cdcl\<^sub>W_twl.conflict (st_of_raw S) (st_of_raw T)"
-proof (cases "raw_conflicting S")
-  case Some
-  then show ?thesis using conf unfolding do_conflict_step_def by simp
-next
-  case None
-  then obtain C where
-    C: "C \<in> set (get_conflict_candidates S)" and
-    T: "T = raw_update_conflicting (Some C) S"
-     using conf unfolding do_conflict_step_def by (auto split: list.splits)
-  have
-    "cls_of_raw_cls C \<in># clauses (st_of_raw S)" and
-    "trail (st_of_raw S) \<Turnstile>as CNot (cls_of_raw_cls C)"
-    using get_conflict_candidates_in_clauses by (simp_all add: C some_in_eq)
-  then show ?thesis
-    using conflict_rule[of "st_of_raw S" "trail (st_of_raw S)" "init_clss (st_of_raw S)"
-      "learned_clss (st_of_raw S)" "backtrack_lvl (st_of_raw S)" "cls_of_raw_cls C" "st_of_raw T"]
-      state_eq_ref T None
-    by (auto simp: conflicting_raw_conflicting)
-qed
+subsubsection \<open>Opaque Type with Invariant\<close>
 
-lemma do_conflict_step_None:
-  assumes conf: "do_conflict_step S = None"
-  shows "no_step conflict (st_of_raw S)"
-proof (cases "conflicting (st_of_raw S)")
-  case Some
-  then show ?thesis by auto
-next
-  case None
-  then have "get_conflict_candidates S = []"
-     using conf unfolding do_conflict_step_def
-     by (auto split: list.splits option.splits simp: conflicting_raw_conflicting)
-  then show ?thesis
-    using get_conflict_candidates_empty by auto
-qed
+declare rough_cdcl.state_simp[simp del]
 
-text \<open>We have a list of conflict candidates, but we take only the first element, in case a conflict
-  appears. This is necessary for non-redundancy.\<close>
-definition do_propagate_step :: "'conc_st \<Rightarrow> 'conc_st option" where
-"do_propagate_step S =
-  (case raw_conflicting S of
-    Some _ \<Rightarrow> None
-  | None \<Rightarrow>
-      (case get_propagate_candidates S of
-        [] \<Rightarrow> None
-      | (L, C) # _ \<Rightarrow> Some (raw_cons_trail (Propagated L C) S)))"
+definition cons_trail_twl :: "('v, nat, 'v twl_clause) marked_lit \<Rightarrow> 'v wf_twl \<Rightarrow> 'v wf_twl"
+  where
+"cons_trail_twl L S \<equiv> twl_of_rough_state (cons_trail L (rough_state_of_twl S))"
 
-lemma do_propagate_step_Some:
-  assumes conf: "do_propagate_step S = Some T"
-  shows "propagate (st_of_raw S) (st_of_raw T)"
-proof (cases "conflicting (st_of_raw S)")
-  case Some
-  then show ?thesis
-    using conf by (auto simp: do_propagate_step_def conflicting_raw_conflicting
-      split: option.splits list.splits)
+lemma wf_twl_state_cons_trail:
+  "undefined_lit (trail S) (lit_of L) \<Longrightarrow> wf_twl_state S \<Longrightarrow> wf_twl_state (cons_trail L S)"
+  unfolding wf_twl_state_def
+  apply (auto simp: cons_trail_def wf_rewatch defined_lit_map
+    comp_def image_def raw_clauses_def)
+  sorry
+
+lemma rough_state_of_twl_cons_trail:
+  "undefined_lit (trail_twl S) (lit_of L) \<Longrightarrow>
+    rough_state_of_twl (cons_trail_twl L S) = cons_trail L (rough_state_of_twl S)"
+  using rough_state_of_twl twl_of_rough_state_inverse wf_twl_state_cons_trail
+  unfolding cons_trail_twl_def by blast
+
+abbreviation add_init_cls_twl where
+"add_init_cls_twl C S \<equiv> twl_of_rough_state (add_init_cls C (rough_state_of_twl S))"
+
+lemma wf_twl_add_init_cls: "wf_twl_state S \<Longrightarrow> wf_twl_state (add_init_cls L S)"
+  unfolding wf_twl_state_def by (auto simp: wf_watch add_init_cls_def split: if_split_asm)
+
+lemma rough_state_of_twl_add_init_cls:
+  "rough_state_of_twl (add_init_cls_twl L S) = add_init_cls L (rough_state_of_twl S)"
+  using rough_state_of_twl twl_of_rough_state_inverse wf_twl_add_init_cls by blast
+
+abbreviation add_learned_cls_twl where
+"add_learned_cls_twl C S \<equiv> twl_of_rough_state (add_learned_cls C (rough_state_of_twl S))"
+
+lemma wf_twl_add_learned_cls: "wf_twl_state S \<Longrightarrow> wf_twl_state (add_learned_cls L S)"
+  unfolding wf_twl_state_def by (auto simp: wf_watch add_learned_cls_def split: if_split_asm)
+
+lemma rough_state_of_twl_add_learned_cls:
+  "rough_state_of_twl (add_learned_cls_twl L S) = add_learned_cls L (rough_state_of_twl S)"
+  using rough_state_of_twl twl_of_rough_state_inverse wf_twl_add_learned_cls by blast
+
+abbreviation remove_cls_twl where
+"remove_cls_twl C S \<equiv> twl_of_rough_state (remove_cls C (rough_state_of_twl S))"
+
+lemma wf_twl_remove_cls: "wf_twl_state S \<Longrightarrow> wf_twl_state (remove_cls L S)"
+  unfolding wf_twl_state_def by (auto simp: wf_watch remove_cls_def split: if_split_asm)
+
+lemma rough_state_of_twl_remove_cls:
+  "rough_state_of_twl (remove_cls_twl L S) = remove_cls L (rough_state_of_twl S)"
+  using rough_state_of_twl twl_of_rough_state_inverse wf_twl_remove_cls by blast
+
+abbreviation init_state_twl where
+"init_state_twl N \<equiv> twl_of_rough_state (init_state N)"
+
+lemma wf_twl_state_wf_twl_state_fold_add_init_cls:
+  assumes "wf_twl_state S"
+  shows "wf_twl_state (fold add_init_cls N S)"
+  using assms apply (induction N arbitrary: S)
+   apply (auto simp: wf_twl_state_def)[]
+  by (simp add: wf_twl_add_init_cls)
+
+lemma wf_twl_state_epsilon_state[simp]:
+  "wf_twl_state (TWL_State [] [] [] 0 None)"
+  by (auto simp: wf_twl_state_def raw_clauses_def)
+
+lemma wf_twl_init_state: "wf_twl_state (init_state N)"
+  unfolding init_state_def by (auto intro!: wf_twl_state_wf_twl_state_fold_add_init_cls)
+
+lemma rough_state_of_twl_init_state:
+  "rough_state_of_twl (init_state_twl N) = init_state N"
+  by (simp add: twl_of_rough_state_inverse wf_twl_init_state)
+
+abbreviation tl_trail_twl where
+"tl_trail_twl S \<equiv> twl_of_rough_state (tl_trail (rough_state_of_twl S))"
+
+lemma wf_twl_state_tl_trail: "wf_twl_state S \<Longrightarrow> wf_twl_state (tl_trail S)"
+  by (auto simp add: twl_of_rough_state_inverse wf_twl_init_state wf_twl_cls_wf_twl_cls_tl
+    tl_trail_def wf_twl_state_def distinct_tl map_tl)
+
+lemma rough_state_of_twl_tl_trail:
+  "rough_state_of_twl (tl_trail_twl S) = tl_trail (rough_state_of_twl S)"
+  using rough_state_of_twl twl_of_rough_state_inverse wf_twl_state_tl_trail by blast
+
+abbreviation update_backtrack_lvl_twl where
+"update_backtrack_lvl_twl k S \<equiv> twl_of_rough_state (update_backtrack_lvl k (rough_state_of_twl S))"
+
+lemma wf_twl_state_update_backtrack_lvl:
+  "wf_twl_state S \<Longrightarrow> wf_twl_state (update_backtrack_lvl k S)"
+  unfolding wf_twl_state_def by auto
+
+lemma rough_state_of_twl_update_backtrack_lvl:
+  "rough_state_of_twl (update_backtrack_lvl_twl k S) = update_backtrack_lvl k
+    (rough_state_of_twl S)"
+  using rough_state_of_twl twl_of_rough_state_inverse wf_twl_state_update_backtrack_lvl by fast
+
+abbreviation update_conflicting_twl where
+"update_conflicting_twl k S \<equiv> twl_of_rough_state (update_conflicting k (rough_state_of_twl S))"
+
+lemma wf_twl_state_update_conflicting:
+  "wf_twl_state S \<Longrightarrow> wf_twl_state (update_conflicting k S)"
+  unfolding wf_twl_state_def by auto
+
+lemma rough_state_of_twl_update_conflicting:
+  "rough_state_of_twl (update_conflicting_twl k S) = update_conflicting k
+    (rough_state_of_twl S)"
+  using rough_state_of_twl twl_of_rough_state_inverse wf_twl_state_update_conflicting by fast
+
+abbreviation raw_clauses_twl where
+"raw_clauses_twl S \<equiv> raw_clauses (rough_state_of_twl S)"
+
+abbreviation restart_twl where
+"restart_twl S \<equiv> twl_of_rough_state (restart' (rough_state_of_twl S))"
+
+lemma wf_wf_restart': "wf_twl_state S \<Longrightarrow> wf_twl_state (restart' S)"
+  unfolding restart'_def wf_twl_state_def apply standard
+   apply clarify
+   apply (rename_tac x)
+   apply (subgoal_tac "wf_twl_cls (trail S) x")
+    apply (case_tac x)
+  using restart_learned by fastforce+
+
+lemma rough_state_of_twl_restart_twl:
+  "rough_state_of_twl (restart_twl S) = restart' (rough_state_of_twl S)"
+  by (simp add: twl_of_rough_state_inverse wf_wf_restart')
+
+(* Sledgehammer is awesome! *)
+interpretation cdcl\<^sub>W_twl_NOT: dpll_state
+  "\<lambda>S. convert_trail_from_W (trail_twl S)"
+  raw_clauses_twl
+  "\<lambda>L S. cons_trail_twl (convert_marked_lit_from_NOT L) S"
+  "\<lambda>S. tl_trail_twl S"
+  "\<lambda>C S. add_learned_cls_twl C S"
+  "\<lambda>C S. remove_cls_twl C S"
+  apply unfold_locales
+         apply (simp add: rough_state_of_twl_cons_trail)
+        apply (metis rough_state_of_twl_tl_trail rough_cdcl.tl_trail)
+       apply (metis rough_state_of_twl_add_learned_cls rough_cdcl.trail_add_cls\<^sub>N\<^sub>O\<^sub>T)
+      apply (metis rough_state_of_twl_remove_cls rough_cdcl.trail_remove_cls)
+     apply (simp add: rough_state_of_twl_cons_trail)
+    apply (simp add: rough_state_of_twl_tl_trail)
+   using rough_cdcl.clauses_add_cls\<^sub>N\<^sub>O\<^sub>T rough_cdcl.clauses_def rough_state_of_twl_add_learned_cls
+   apply auto[1]
+  using rough_cdcl.clauses_def rough_cdcl.clauses_remove_cls rough_state_of_twl_remove_cls by auto
+
+interpretation cdcl\<^sub>W_twl: state\<^sub>W
+  trail_twl
+  init_clss_twl
+  learned_clss_twl
+  backtrack_lvl_twl
+  conflicting_twl
+  cons_trail_twl
+  tl_trail_twl
+  add_init_cls_twl
+  add_learned_cls_twl
+  remove_cls_twl
+  update_backtrack_lvl_twl
+  update_conflicting_twl
+  init_state_twl
+  restart_twl
+  apply unfold_locales
+  by (simp_all add: rough_state_of_twl_cons_trail rough_state_of_twl_tl_trail
+    rough_state_of_twl_add_init_cls rough_state_of_twl_add_learned_cls rough_state_of_twl_remove_cls
+    rough_state_of_twl_update_backtrack_lvl rough_state_of_twl_update_conflicting
+    rough_state_of_twl_init_state rough_state_of_twl_restart_twl
+    rough_cdcl.learned_clss_restart_state)
+
+interpretation cdcl\<^sub>W_twl: cdcl\<^sub>W
+  trail_twl
+  init_clss_twl
+  learned_clss_twl
+  backtrack_lvl_twl
+  conflicting_twl
+  cons_trail_twl
+  tl_trail_twl
+  add_init_cls_twl
+  add_learned_cls_twl
+  remove_cls_twl
+  update_backtrack_lvl_twl
+  update_conflicting_twl
+  init_state_twl
+  restart_twl
+  by unfold_locales
+
+sublocale cdcl\<^sub>W
+  trail_twl
+  init_clss_twl
+  learned_clss_twl
+  backtrack_lvl_twl
+  conflicting_twl
+  cons_trail_twl
+  tl_trail_twl
+  add_init_cls_twl
+  add_learned_cls_twl
+  remove_cls_twl
+  update_backtrack_lvl_twl
+  update_conflicting_twl
+  init_state_twl
+  restart_twl
+  by (rule cdcl\<^sub>W_twl.cdcl\<^sub>W_axioms)
+
+abbreviation state_eq_twl (infix "\<sim>TWL" 51) where
+"state_eq_twl S S' \<equiv> rough_cdcl.state_eq (rough_state_of_twl S) (rough_state_of_twl S')"
+notation cdcl\<^sub>W_twl.state_eq (infix "\<sim>" 51)
+declare cdcl\<^sub>W_twl.state_simp[simp del]
+  cdcl\<^sub>W_twl_NOT.state_simp\<^sub>N\<^sub>O\<^sub>T[simp del]
+
+text \<open>To avoid ambiguities:\<close>
+no_notation state_eq_twl (infix "\<sim>" 51)
+
+definition propagate_twl where
+"propagate_twl S S' \<longleftrightarrow>
+  (\<exists>L C. (L, C) \<in> candidates_propagate_twl S
+  \<and> S' \<sim> cons_trail_twl (Propagated L C) S
+  \<and> conflicting_twl S = None)"
+
+lemma propagate_twl_iff_propagate:
+  assumes inv: "cdcl\<^sub>W_twl.cdcl\<^sub>W_all_struct_inv S"
+  shows "cdcl\<^sub>W_twl.propagate S T \<longleftrightarrow> propagate_twl S T" (is "?P \<longleftrightarrow> ?T")
+proof
+  assume ?P
+  then obtain C L where
+    "conflicting (rough_state_of_twl S) = None" and
+    CL_Clauses: "C + {#L#} \<in># cdcl\<^sub>W_twl.clauses S" and
+    tr_CNot: "trail_twl S \<Turnstile>as CNot C" and
+    undef_lot: "undefined_lit (trail_twl S) L" and
+    "T \<sim> cons_trail_twl (Propagated L (C + {#L#})) S"
+    unfolding cdcl\<^sub>W_twl.propagate.simps by blast
+  have "distinct_mset (C + {#L#})"
+    using inv CL_Clauses unfolding cdcl\<^sub>W_twl.cdcl\<^sub>W_all_struct_inv_def
+    cdcl\<^sub>W_twl.distinct_cdcl\<^sub>W_state_def cdcl\<^sub>W_twl.clauses_def distinct_mset_set_def
+    by auto
+  then have C_L_L: "mset_set (set_mset (C + {#L#}) - {L}) = C"
+    by (metis Un_insert_right add_diff_cancel_left' add_diff_cancel_right'
+      distinct_mset_set_mset_ident finite_set_mset insert_absorb2 mset_set.insert_remove
+      set_mset_single set_mset_union)
+  have "(L, C+{#L#}) \<in> candidates_propagate_twl S"
+    apply (rule wf_candidates_propagate_complete)
+         using rough_state_of_twl apply auto[]
+        using CL_Clauses unfolding cdcl\<^sub>W_twl.clauses_def apply auto[]
+       apply simp
+      using C_L_L tr_CNot apply simp
+     using undef_lot apply blast
+     done
+  show ?T unfolding propagate_twl_def
+    apply (rule exI[of _ "L"], rule exI[of _ "C+{#L#}"])
+    apply (auto simp: \<open>(L, C+{#L#}) \<in> candidates_propagate_twl S\<close>
+      \<open>conflicting (rough_state_of_twl S) = None\<close> )
+    using \<open>T \<sim> cons_trail_twl (Propagated L (C + {#L#})) S\<close> cdcl\<^sub>W_twl.state_eq_backtrack_lvl
+    cdcl\<^sub>W_twl.state_eq_conflicting cdcl\<^sub>W_twl.state_eq_init_clss
+    cdcl\<^sub>W_twl.state_eq_learned_clss cdcl\<^sub>W_twl.state_eq_trail rough_cdcl.state_eq_def by blast
 next
-  case None
+  assume ?T
   then obtain L C where
-    C: "(L, C) \<in> set (get_propagate_candidates S)" and
-    T: "T = raw_cons_trail (Propagated L C) S"
-     using conf unfolding do_propagate_step_def
-    by (auto split: list.splits simp: conflicting_raw_conflicting)
-  have
-    "cls_of_raw_cls C \<in># clauses (st_of_raw S)" and
-    undef: "undefined_lit (trail (st_of_raw S)) L"
-    "trail (st_of_raw S) \<Turnstile>as CNot (cls_of_raw_cls C - {#L#})" and
-    "L \<in># cls_of_raw_cls C"
-    using get_propagate_candidates_lit_in_cls C by auto
-  then show ?thesis
-    using propagate_rule[of "st_of_raw S" "trail (st_of_raw S)" "init_clss (st_of_raw S)"
-      "learned_clss (st_of_raw S)" "backtrack_lvl (st_of_raw S)" "cls_of_raw_cls C - {#L#}" L
-      "st_of_raw T"]
-      state_eq_ref T None
-    by (auto simp: conflicting_raw_conflicting)
-qed
+    LC: "(L, C) \<in> candidates_propagate_twl S" and
+    T: "T \<sim> cons_trail_twl (Propagated L C) S" and
+    confl: "conflicting (rough_state_of_twl S) = None"
+    unfolding propagate_twl_def by auto
+  have [simp]: "C - {#L#} + {#L#} = C"
+    using LC unfolding candidates_propagate_def
+    by clarify (metis Multiset.diff_le_self insert_DiffM2 mset_leD multi_member_last union_iff)
+  have "C \<in># raw_clauses_twl S"
+    using LC unfolding candidates_propagate_def rough_cdcl.clauses_def by auto
+  then have "distinct_mset C"
+    using inv unfolding cdcl\<^sub>W_twl.cdcl\<^sub>W_all_struct_inv_def cdcl\<^sub>W_twl.distinct_cdcl\<^sub>W_state_def
+    cdcl\<^sub>W_twl.clauses_def distinct_mset_set_def rough_cdcl.clauses_def by auto
+  then have C_L_L: "mset_set (set_mset C - {L}) = C - {#L#}"
+    by (metis \<open>C - {#L#} + {#L#} = C\<close> add_left_imp_eq diff_single_trivial
+      distinct_mset_set_mset_ident finite_set_mset mset_set.remove
+      multi_self_add_other_not_self union_commute)
 
-lemma do_propagate_step_None:
-  assumes conf: "do_propagate_step S = None"
-  shows "no_step propagate (st_of_raw S)"
-proof (cases "conflicting (st_of_raw S)")
-  case Some
-  then show ?thesis by auto
+  show ?P
+    apply (rule cdcl\<^sub>W_twl.propagate.intros[of _ "trail_twl S" "init_clss_twl S"
+      "learned_clss_twl S" "backtrack_lvl_twl S" "C-{#L#}" L])
+        using confl apply auto[]
+       using LC unfolding candidates_propagate_def apply (auto simp: cdcl\<^sub>W_twl.clauses_def)[]
+      using wf_candidates_propagate_sound[OF _ LC] rough_state_of_twl apply (simp add: C_L_L)
+     using wf_candidates_propagate_sound[OF _ LC] rough_state_of_twl apply simp
+    using T unfolding cdcl\<^sub>W_twl.state_eq_def rough_cdcl.state_eq_def by auto
+qed
+no_notation CDCL_Two_Watched_Literals.twl.state_eq_twl (infix "\<sim>TWL" 51)
+definition conflict_twl where
+"conflict_twl S S' \<longleftrightarrow>
+  (\<exists>C. C \<in> candidates_conflict_twl S
+  \<and> S' \<sim> update_conflicting_twl (Some C) S
+  \<and> conflicting_twl S = None)"
+
+lemma conflict_twl_iff_conflict:
+  shows "cdcl\<^sub>W_twl.conflict S T \<longleftrightarrow> conflict_twl S T" (is "?C \<longleftrightarrow> ?T")
+proof
+  assume ?C
+  then obtain M N U k C where
+    S: "rough_cdcl.state (rough_state_of_twl S) = (M, N, U, k, None)" and
+    C: "C \<in># cdcl\<^sub>W_twl.clauses S" and
+    M_C: "M \<Turnstile>as CNot C" and
+    T: "T \<sim> update_conflicting_twl (Some C) S"
+    by auto
+  have "C \<in> candidates_conflict_twl S"
+    apply (rule wf_candidates_conflict_complete)
+       apply simp
+      using C apply (auto simp: cdcl\<^sub>W_twl.clauses_def)[]
+    using M_C S by auto
+  moreover have "T \<sim> twl_of_rough_state (update_conflicting (Some C) (rough_state_of_twl S))"
+    using T unfolding rough_cdcl.state_eq_def cdcl\<^sub>W_twl.state_eq_def by auto
+  ultimately show ?T
+    using S unfolding conflict_twl_def by auto
 next
-  case None
-  then have "get_propagate_candidates S = []"
-     using conf unfolding do_propagate_step_def
-     by (auto split: list.splits option.splits simp: conflicting_raw_conflicting)
-  then show ?thesis
-    unfolding get_propagate_candidates_empty by (force elim!: propagateE)
+  assume ?T
+  then obtain C where
+    C: "C \<in> candidates_conflict_twl S" and
+    T: "T \<sim> update_conflicting_twl (Some C) S" and
+    confl: "conflicting_twl S = None"
+    unfolding conflict_twl_def by auto
+  have "C \<in># cdcl\<^sub>W_twl.clauses S"
+    using C unfolding candidates_conflict_def cdcl\<^sub>W_twl.clauses_def by auto
+ moreover have "trail_twl S \<Turnstile>as CNot C"
+    using wf_candidates_conflict_sound[OF _ C] by auto
+ ultimately show ?C apply -
+   apply (rule cdcl\<^sub>W_twl.conflict.conflict_rule[of _ _ _ _ _ C])
+   using confl T unfolding rough_cdcl.state_eq_def cdcl\<^sub>W_twl.state_eq_def by auto
 qed
 
-definition do_skip_step :: "'conc_st \<Rightarrow> 'conc_st option"  where
-"do_skip_step S =
-  (case conflicting (st_of_raw S) of
-    None \<Rightarrow> None
-  | Some D \<Rightarrow>
-    (case trail (st_of_raw S) of
-      Propagated L C' # _ \<Rightarrow>
-        if -L \<notin># D \<and> D \<noteq> {#} then Some (raw_tl_trail S) else None
-    | _ \<Rightarrow> None))"
+inductive cdcl\<^sub>W_twl :: "'v wf_twl \<Rightarrow> 'v wf_twl \<Rightarrow> bool" for S :: "'v wf_twl" where
+propagate: "propagate_twl S S' \<Longrightarrow> cdcl\<^sub>W_twl S S'" |
+conflict: "conflict_twl S S' \<Longrightarrow> cdcl\<^sub>W_twl S S'" |
+other: "cdcl\<^sub>W_twl.cdcl\<^sub>W_o S S' \<Longrightarrow> cdcl\<^sub>W_twl S S'"|
+rf: "cdcl\<^sub>W_twl.cdcl\<^sub>W_rf S S' \<Longrightarrow> cdcl\<^sub>W_twl S S'"
 
-lemma do_skip_step_Some:
-  assumes conf: "do_skip_step S = Some T"
-  shows "skip (st_of_raw S) (st_of_raw T)"
-proof (cases "conflicting (st_of_raw S)")
-  case None
-  then show ?thesis
-    using conf by (auto simp: do_skip_step_def)
+lemma cdcl\<^sub>W_twl_iff_cdcl\<^sub>W:
+  assumes "cdcl\<^sub>W_twl.cdcl\<^sub>W_all_struct_inv S"
+  shows "cdcl\<^sub>W_twl S T \<longleftrightarrow> cdcl\<^sub>W_twl.cdcl\<^sub>W S T"
+  by (simp add: assms cdcl\<^sub>W_twl.cdcl\<^sub>W.simps cdcl\<^sub>W_twl.simps conflict_twl_iff_conflict
+    propagate_twl_iff_propagate)
+
+lemma rtranclp_cdcl\<^sub>W_twl_all_struct_inv_inv:
+  assumes "cdcl\<^sub>W_twl\<^sup>*\<^sup>* S T" and "cdcl\<^sub>W_twl.cdcl\<^sub>W_all_struct_inv S"
+  shows "cdcl\<^sub>W_twl.cdcl\<^sub>W_all_struct_inv T"
+  using assms by (induction rule: rtranclp_induct)
+  (simp_all add: cdcl\<^sub>W_twl_iff_cdcl\<^sub>W cdcl\<^sub>W_twl.cdcl\<^sub>W_all_struct_inv_inv)
+
+lemma rtranclp_cdcl\<^sub>W_twl_iff_rtranclp_cdcl\<^sub>W:
+  assumes "cdcl\<^sub>W_twl.cdcl\<^sub>W_all_struct_inv S"
+  shows "cdcl\<^sub>W_twl\<^sup>*\<^sup>* S T \<longleftrightarrow> cdcl\<^sub>W_twl.cdcl\<^sub>W\<^sup>*\<^sup>* S T" (is "?T \<longleftrightarrow> ?W")
+proof
+  assume ?W
+  then show ?T
+    proof (induction rule: rtranclp_induct)
+      case base
+      then show ?case by simp
+    next
+      case (step T U) note st = this(1) and cdcl = this(2) and IH = this(3)
+      have "cdcl\<^sub>W_twl T U"
+        using assms st cdcl cdcl\<^sub>W_twl.rtranclp_cdcl\<^sub>W_all_struct_inv_inv cdcl\<^sub>W_twl_iff_cdcl\<^sub>W
+        by blast
+      then show ?case using IH by auto
+    qed
 next
-  case (Some D)
-  then obtain L C M  where
-    C: "trail (st_of_raw S) = Propagated L C # M" and
-    T: " -L \<notin># D" and
-    "D \<noteq> {#}" and
-    "st_of_raw T = tl_trail (st_of_raw S)"
-    using conf unfolding do_skip_step_def
-    by (auto split: list.splits marked_lit.splits if_split_asm simp: conflicting_raw_conflicting)
-  then show ?thesis
-    using skip_rule[of "st_of_raw S" L C M "init_clss (st_of_raw S)"
-      "learned_clss (st_of_raw S)" "backtrack_lvl (st_of_raw S)"]
-      state_eq_ref T Some
-    by (auto simp: conflicting_raw_conflicting)
+  assume ?T
+  then show ?W
+    proof (induction rule: rtranclp_induct)
+      case base
+      then show ?case by simp
+    next
+      case (step T U) note st = this(1) and cdcl = this(2) and IH = this(3)
+      have "cdcl\<^sub>W_twl.cdcl\<^sub>W T U"
+        using assms st cdcl rtranclp_cdcl\<^sub>W_twl_all_struct_inv_inv cdcl\<^sub>W_twl_iff_cdcl\<^sub>W
+        by blast
+      then show ?case using IH by auto
+    qed
 qed
 
-lemma do_skip_step_None:
-  assumes conf: "do_skip_step S = None"
-  shows "no_step skip (st_of_raw S)"
-proof (cases "conflicting (st_of_raw S)")
-  case None
-  then show ?thesis by auto
-next
-  case Some
-  then show ?thesis
-    using conf unfolding do_skip_step_def
-    by (auto split: list.splits marked_lit.splits if_split_asm simp: conflicting_raw_conflicting)
+interpretation cdcl\<^sub>N\<^sub>O\<^sub>T_twl: backjumping_ops
+  "\<lambda>S. convert_trail_from_W (trail_twl S)"
+  abstract_twl.raw_clauses_twl
+  "\<lambda>L (S:: 'v wf_twl).
+    cons_trail_twl
+      (convert_marked_lit_from_NOT L) (S:: 'v wf_twl)"
+  tl_trail_twl
+  add_learned_cls_twl
+  remove_cls_twl
+  (* bj conditions *) "\<lambda>C _ _ (S:: 'v wf_twl) _. C \<in> candidates_conflict_twl S"
+  by unfold_locales
+
+lemma reduce_trail_to\<^sub>N\<^sub>O\<^sub>T_skip_beginning_twl:
+  assumes "trail_twl S = convert_trail_from_NOT (F' @ F)"
+  shows "trail_twl (cdcl\<^sub>W_twl.reduce_trail_to\<^sub>N\<^sub>O\<^sub>T F S) = convert_trail_from_NOT F"
+  using assms by (induction F' arbitrary: S) auto
+
+lemma reduce_trail_to\<^sub>N\<^sub>O\<^sub>T_trail_tl_trail_twl_decomp[simp]:
+  "trail_twl S = convert_trail_from_NOT (F' @ Marked K () # F) \<Longrightarrow>
+     trail_twl (cdcl\<^sub>W_twl.reduce_trail_to\<^sub>N\<^sub>O\<^sub>T F (tl_trail_twl S)) = convert_trail_from_NOT F"
+  apply (rule reduce_trail_to\<^sub>N\<^sub>O\<^sub>T_skip_beginning_twl[of _ "tl (F' @ Marked K () # [])"])
+  by (cases F') (auto simp add:tl_append rough_cdcl.reduce_trail_to\<^sub>N\<^sub>O\<^sub>T_skip_beginning)
+
+lemma trail_twl_reduce_trail_to\<^sub>N\<^sub>O\<^sub>T_drop:
+  "trail_twl (cdcl\<^sub>W_twl.reduce_trail_to\<^sub>N\<^sub>O\<^sub>T F S) =
+    (if length (trail_twl S) \<ge> length F
+    then drop (length (trail_twl S) - length F) (trail_twl S)
+    else [])"
+  apply (induction F S rule: cdcl\<^sub>W_twl.reduce_trail_to\<^sub>N\<^sub>O\<^sub>T.induct)
+  apply (rename_tac F S)
+  apply (case_tac "trail_twl S")
+   apply auto[]
+  apply (rename_tac list)
+  apply (case_tac "Suc (length list) > length F")
+   prefer 2 apply simp
+  apply (subgoal_tac "Suc (length list) - length F = Suc (length list - length F)")
+   apply simp
+  apply simp
+  done
+
+interpretation cdcl\<^sub>N\<^sub>O\<^sub>T_twl: dpll_with_backjumping_ops
+  "\<lambda>S. convert_trail_from_W (trail_twl S)"
+  abstract_twl.raw_clauses_twl
+  "\<lambda>L S.
+    cons_trail_twl
+      (convert_marked_lit_from_NOT L) S"
+  tl_trail_twl
+  add_learned_cls_twl
+  remove_cls_twl
+  (* propagate conditions: *)"\<lambda>L S. lit_of L \<in> fst ` candidates_propagate_twl S"
+  (* state invariant *)"\<lambda>S. no_dup (trail_twl S)"
+  (* backjump conditions *)"\<lambda>C _ _ S _. C \<in> candidates_conflict_twl S"
+proof (unfold_locales, goal_cases)
+  case (1 C' S C F' K F L) note n_d = this(1) and n_d' = this(2) and undef = this(6)
+  let ?T' = "(cons_trail (Propagated L {#}) (rough_state_of_twl (cdcl\<^sub>W_twl.reduce_trail_to\<^sub>N\<^sub>O\<^sub>T F S)))"
+  let ?T = "(cons_trail_twl (Propagated L {#}) (cdcl\<^sub>W_twl.reduce_trail_to\<^sub>N\<^sub>O\<^sub>T F S))"
+  have tr_F_S: "map lit_of (trail_twl (cdcl\<^sub>W_twl.reduce_trail_to\<^sub>N\<^sub>O\<^sub>T F S)) =
+    map lit_of (convert_trail_from_NOT F)"
+    apply (subst trail_twl_reduce_trail_to\<^sub>N\<^sub>O\<^sub>T_drop[of F S])
+    using 1(1) arg_cong[OF 1(3), of length] arg_cong[OF 1(3), of "map lit_of"]
+    by (auto simp: o_def drop_map[symmetric])
+
+  have "no_dup (trail_twl S)"
+    using "1"(1) by blast
+  have "wf_twl_state (rough_state_of_twl (cdcl\<^sub>W_twl.reduce_trail_to\<^sub>N\<^sub>O\<^sub>T F S))"
+    using wf_twl_state_rough_state_of_twl by blast
+  moreover have undef': "undefined_lit (trail_twl (cdcl\<^sub>W_twl.reduce_trail_to\<^sub>N\<^sub>O\<^sub>T F S)) L"
+    using undef arg_cong[OF tr_F_S, of "map atm_of"] unfolding defined_lit_map image_set
+    by (simp add:  o_def)
+  ultimately have "wf_twl_state ?T'"
+    by (simp_all add: wf_twl_state_cons_trail)
+  then have "init_clss_twl ?T = init_clss_twl (cdcl\<^sub>W_twl.reduce_trail_to\<^sub>N\<^sub>O\<^sub>T F S)"
+      using 1(6) by (simp add: undef')
+  then have [simp]: "init_clss_twl ?T = init_clss_twl S"
+     by (simp add: cdcl\<^sub>W_twl.reduce_trail_to\<^sub>N\<^sub>O\<^sub>T_reduce_trail_convert)
+
+  have "learned_clss_twl ?T = learned_clss_twl (cdcl\<^sub>W_twl.reduce_trail_to\<^sub>N\<^sub>O\<^sub>T F S)"
+    by (smt "1"(3) "1"(6) append_assoc cdcl\<^sub>W_twl.learned_clss_cons_trail
+      cdcl\<^sub>W_twl_NOT.reduce_trail_to\<^sub>N\<^sub>O\<^sub>T_eq_length cdcl\<^sub>W_twl_NOT.reduce_trail_to\<^sub>N\<^sub>O\<^sub>T_nil
+      cdcl\<^sub>W_twl_NOT.reduce_trail_to\<^sub>N\<^sub>O\<^sub>T_skip_beginning comp_apply defined_lit_convert_trail_from_W
+      list.sel(3) marked_lit.sel(2) rev.simps(2) rev_append rev_eq_Cons_iff
+      cons_trail_twl_def)
+  moreover have "learned_clss_twl (cdcl\<^sub>W_twl.reduce_trail_to\<^sub>N\<^sub>O\<^sub>T F S)
+    = learned_clss_twl S"
+    by (simp add: cdcl\<^sub>W_twl.reduce_trail_to\<^sub>N\<^sub>O\<^sub>T_reduce_trail_convert)
+  ultimately have [simp]: "learned_clss_twl ?T = learned_clss_twl S"
+    by simp
+  have tr_L_F_S: "map lit_of (trail_twl ?T)
+    = map lit_of (Propagated L {#} # convert_trail_from_NOT F)"
+    using undef' tr_F_S by (simp add: o_def)
+  have C_confl_cand: "C \<in> candidates_conflict_twl S"
+    apply(rule wf_candidates_twl_conflict_complete)
+     using 1(1,4) apply (simp add: rough_cdcl.clauses_def)
+    using 1(5) by (simp add: tr_L_F_S true_annots_true_cls lits_of_l_convert_trail_from_NOT)
+
+  have "cdcl\<^sub>N\<^sub>O\<^sub>T_twl.backjump S
+    (cons_trail_twl (convert_marked_lit_from_NOT (Propagated L ()))
+      (cdcl\<^sub>W_twl.reduce_trail_to\<^sub>N\<^sub>O\<^sub>T F S))"
+    apply (rule cdcl\<^sub>N\<^sub>O\<^sub>T_twl.backjump.intros[of S F' K F _ L C, OF 1(3) _ 1(4-6) _ 1(8-9)])
+      unfolding cdcl\<^sub>W_twl_NOT.state_eq\<^sub>N\<^sub>O\<^sub>T_def apply (metis convert_marked_lit_from_NOT.simps(1))
+     using 1(7) 1(3) apply presburger
+    using C_confl_cand by simp
+  then show ?case
+    by blast
 qed
 
-definition do_resolve_step :: "'conc_st \<Rightarrow> 'conc_st option" where
-"do_resolve_step S =
-  (case raw_conflicting S of
-    None \<Rightarrow> None
-  | Some D \<Rightarrow>
-    if trail (st_of_raw S) \<noteq> []
-    then
-      (case raw_hd_trail S of
-        Propagated L C \<Rightarrow>
-          if -L \<in># cls_of_raw_cls D \<and> cls_of_raw_cls D \<noteq> {#} \<and>
-             maximum_level (remove (-L) D) S = raw_backtrack_lvl S
-          then Some (raw_update_conflicting
-             (Some (raw_cls_union (remove (-L) D) (remove L C)))
-             (raw_tl_trail S))
-          else None
-      | _ \<Rightarrow> None)
-    else None)"
+interpretation cdcl\<^sub>N\<^sub>O\<^sub>T_twl: dpll_with_backjumping
+  "\<lambda>S. convert_trail_from_W (trail_twl S)"
+  abstract_twl.raw_clauses_twl
+  "\<lambda>L (S:: 'v wf_twl).
+    cons_trail_twl
+      (convert_marked_lit_from_NOT L) (S:: 'v wf_twl)"
+  tl_trail_twl
+  add_learned_cls_twl
+  remove_cls_twl
+  (* propagate conditions: *)"\<lambda>L S. lit_of L \<in> fst ` candidates_propagate_twl S"
+  (* state invariant *)"\<lambda>S. no_dup (trail_twl S)"
+  (* backjump conditions *)"\<lambda>C _ _ (S:: 'v wf_twl) _. C \<in> candidates_conflict_twl S"
+  apply unfold_locales
+  using cdcl\<^sub>N\<^sub>O\<^sub>T_twl.dpll_bj_no_dup by (simp add: o_def)
+end
 
-
-lemma do_resolve_step_Some:
-  assumes conf: "do_resolve_step S = Some T" and inv: "cdcl\<^sub>W_all_struct_inv (st_of_raw S)"
-  shows "resolve (st_of_raw S) (st_of_raw T)"
-proof (cases "raw_conflicting S")
-  case None
-  then show ?thesis
-    using conf by (auto simp: do_resolve_step_def)
-next
-  case (Some D)
-  def M \<equiv> "tl (trail (st_of_raw S))"
-  obtain L C where
-    C: "raw_hd_trail S = Propagated L C" and
-    T: " -L \<in># cls_of_raw_cls D" and
-    "cls_of_raw_cls D \<noteq> {#}" and
-    "T =
-      raw_update_conflicting (Some (raw_cls_union (remove (-L) D) (remove L C))) (raw_tl_trail S)" and
-    "maximum_level (remove (-L) D) S = raw_backtrack_lvl S" and
-    empty: "trail (st_of_raw S) \<noteq> []"
-    using conf Some unfolding do_resolve_step_def
-    by (auto split: list.splits marked_lit.splits if_split_asm simp: conflicting_raw_conflicting)
-  moreover have "trail (st_of_raw S) = Propagated L (cls_of_raw_cls C) # M"
-    using empty raw_hd_trail[of S] C M_def by (cases "trail (st_of_raw S)") simp_all
-  moreover then have "L \<in># cls_of_raw_cls C"
-    using inv unfolding  cdcl\<^sub>W_all_struct_inv_def cdcl\<^sub>W_conflicting_def by force
-  ultimately show ?thesis
-    using resolve_rule[of "st_of_raw S" L "cls_of_raw_cls C - {#L#}" "tl (trail (st_of_raw S))"
-      "init_clss (st_of_raw S)"
-      "learned_clss (st_of_raw S)" "backtrack_lvl (st_of_raw S)" "cls_of_raw_cls D - {#-L#}"
-      "st_of_raw T"]
-      state_eq_ref T Some
-    by (auto simp: conflicting_raw_conflicting raw_backtrack_lvl)
-qed
-
-definition do_backtrack_step :: "'conc_st \<Rightarrow> 'conc_st option" where
-"do_backtrack_step S = None"
-
-definition do_bj_step :: "'conc_st \<Rightarrow> 'conc_st option" where
-"do_bj_step S =
-  (case do_skip_step S of
-    Some T \<Rightarrow> Some T
-  | None \<Rightarrow>
-    (case do_resolve_step S of
-      Some T \<Rightarrow> Some T
-    | None \<Rightarrow> do_backtrack_step S))"
- *)
 end
